Housekeeping

specIR/SIRcommon.v
@@ -19,109 +19,16 @@ Require Import Mod ModSem Any Skeleton.
 Require Import Program.
 Require Import Simulation.
 Require Import AxiomsC.
+Require Export ITreelib.
 
 Set Implicit Arguments.
 Set Universe Polymorphism.
-
-From ExtLib Require Export
-     (* Data.String *)
-     (* Structures.Monad *)
-     (* Structures.Traversable *)
-     (* Structures.Foldable *)
-     (* Structures.Reducible *)
-     (* OptionMonad *)
-     Functor FunctorLaws
-     Structures.Maps
-     (* Data.List *)
-.
-
-From ITree Require Export
-     ITree
-     ITreeFacts
-     Events.MapDefault
-     Events.State
-     Events.StateFacts
-     EqAxiom
-.
-
-Export SumNotations.
-Export ITreeNotations.
-Export Monads.
-Export MonadNotation.
-Export FunctorNotation.
-Open Scope monad_scope.
-Open Scope itree_scope.
-(* Notation "` x : t <- t1 ;; t2" := (ITree.bind t1 (fun x : t => t2)) *)
-(*   (at level 61, t at next level, t1 at next level, x ident, right associativity) : itree_scope. *)
-
-
-
-
-Instance function_Map (K V: Type) (dec: forall k0 k1, {k0=k1} + {k0<>k1}): (Map K V (K -> option V)) :=
-  Build_Map
-    (fun _ => None)
-    (fun k0 v m => fun k1 => if dec k0 k1 then Some v else m k1)
-    (fun k0 m => fun k1 => if dec k0 k1 then None else m k1)
-    (fun k m => m k)
-    (fun m0 m1 => fun k => match (m0 k) with
-                           | Some v => Some v
-                           | _ => m1 k
-                           end)
-.
-
-
-Lemma eq_eutt
-      E R
-      (a b: itree E R)
-      (EQ: a = b)
-  :
-    eutt eq a b
-.
-Proof. i. clarify. refl. Qed.
-
-Lemma vis_not_ret
-      E R (r: R) X (e: E X) k
-      (EUTT: Vis e k ≈ Ret r)
-  :
-    False
-.
-Proof. ii. punfold EUTT. inv EUTT. Qed.
-
-(* Lemma eqit_inv_vis {E R1 R2 RR} b1 b2 {u1 u2} (e1: E u1) (e2: E u2) *)
-(*       (k1: u1 -> itree E R1) (k2: u2 -> itree E R2) : *)
-(*   eqit RR b1 b2 (Vis e1 k1) (Vis e2 k2) -> *)
-(*   u1 = u2 /\ e1 ~= e2 /\ (forall u1 u2 (EQ: u1 ~= u2), eqit RR b1 b2 (k1 u1) (k2 u2)). *)
-(* Proof. *)
-(*   intros. punfold H. repeat red in H. simpl in H. *)
-(*   dependent destruction H. pclearbot. esplits; eauto. *)
-(*   ii. apply JMeq_eq in EQ. clarify. *)
-(* Qed. *)
-
-Fail Lemma empty_nonempty
-      (T: Type)
-      (EQ: void = T)
-      (INHAB: inhabited T)
-  :
-    False
-.
-(* Proof. *)
-(*   inversion INHAB. rewrite <- EQ in H. inv H. *)
-(* Qed. *)
-
-
-
-
-
 
 
 
 Section OWNEDHEAP.
 
 Variable owned_heap: Type.
-
-
-
-
 
 Section EFF.
 
@@ -201,7 +108,7 @@ Section DENOTE.
       end
   .
 
-  Definition interp_program0:
+  Definition interp_program:
     (forall T, InternalCallE T -> itree eff0 T) :=
     fun _ ic =>
       let sem0: itree eff0 _ := (mrec interp_function) _ ic in
@@ -239,7 +146,7 @@ Definition global_definitions: list (ident * globdef (fundef (function)) unit) :
 Definition p: program := Maps.add _sum c_sum (Maps.empty).
 
 Variable initial_oh: owned_heap.
-Let one := (interp_program0 p (ICall _sum initial_oh Mem.empty [Vint (Int.repr 1%Z)])).
+Let one := (interp_program p (ICall _sum initial_oh Mem.empty [Vint (Int.repr 1%Z)])).
 (* Compute (burn 1 one). *)
 
 Lemma one_spec
@@ -247,7 +154,7 @@ Lemma one_spec
     one ≈ Ret (initial_oh, (Mem.empty, Vint (Int.repr 1%Z)))
 .
 Proof.
-  subst one. unfold interp_program0. ss.
+  subst one. unfold interp_program. ss.
   rewrite mrec_as_interp. cbn. des_ifs. cbn. des_ifs.
   autorewrite with itree. cbn.
   rewrite mrec_as_interp. cbn. des_ifs. cbn. des_ifs.
@@ -261,72 +168,6 @@ End TEST.
 
 End OWNEDHEAP.
 
-
-
-Lemma eq_is_bisim: forall E R (t1 t2 : itree E R), t1 = t2 -> t1 ≅ t2.
-Proof. ii. clarify. reflexivity. Qed.
-Lemma bisim_is_eq: forall E R (t1 t2 : itree E R), t1 ≅ t2 -> t1 = t2.
-Proof. ii. eapply bisimulation_is_eq; eauto. Qed.
-
-
-
-Ltac f := first [eapply bisim_is_eq|eapply eq_is_bisim].
-Tactic Notation "f" "in" hyp(H) := first [eapply bisim_is_eq in H|eapply eq_is_bisim in H].
-Ltac ides itr :=
-  let T := fresh "T" in
-  destruct (observe itr) eqn:T;
-  sym in T; apply simpobs in T; apply bisim_is_eq in T; rewrite T in *; clarify.
-Ltac csc := clarify; simpl_depind; clarify.
-
-Notation "tau;; t2" := (Tau t2)
-  (at level 200, right associativity) : itree_scope.
-
-
-
-(*** COPIED FROM MASTER BRANCH. REMOVE LATER ***)
-(*** COPIED FROM MASTER BRANCH. REMOVE LATER ***)
-(*** COPIED FROM MASTER BRANCH. REMOVE LATER ***)
-Lemma eutt_eq_bind : forall E R U (t1 t2: itree E U) (k1 k2: U -> itree E R), t1 ≈ t2 -> (forall u, k1 u ≈ k2 u) -> ITree.bind t1 k1 ≈ ITree.bind t2 k2.
-Proof.
-  intros.
-  eapply eutt_clo_bind with (UU := Logic.eq); [eauto |].
-  intros ? ? ->. apply H0.
-Qed.
-Ltac f_equiv := first [eapply eutt_eq_bind|eapply eqit_VisF|Morphisms.f_equiv].
-(* eapply eqit_bind'| *)
-
-Hint Rewrite @bind_trigger : itree.
-Hint Rewrite @tau_eutt : itree.
-Hint Rewrite @bind_tau : itree.
-
-Tactic Notation "irw" "in" ident(H) := repeat (autorewrite with itree in H; cbn in H).
-Tactic Notation "irw" := repeat (autorewrite with itree; cbn).
-
-(*** TODO: IDK why but (1) ?UNUSNED is needed (2) "fold" tactic does not work. WHY????? ***)
-Ltac fold_eutt :=
-  repeat multimatch goal with
-         | [ H: eqit eq true true ?A ?B |- ?UNUSED ] =>
-           let name := fresh "tmp" in
-           assert(tmp: eutt eq A B) by apply H; clear H; rename tmp into H
-         end
-.
-
-Lemma bind_ret_map {E R1 R2} (u : itree E R1) (f : R1 -> R2) :
-  (r <- u ;; Ret (f r)) ≅ f <$> u.
-Proof.
-  rewrite <- (bind_ret_r u) at 2. apply eqit_bind.
-  - hnf. intros. apply eqit_Ret. auto.
-  - rewrite bind_ret_r. reflexivity.
-Qed.
-
-Lemma map_vis {E R1 R2 X} (e: E X) (k: X -> itree E R1) (f: R1 -> R2) :
-  (* (f <$> (Vis e k)) ≅ Vis e (fun x => f <$> (k x)). *)
-  ITree.map f (Vis e k) ≅ Vis e (fun x => f <$> (k x)).
-Proof.
-  cbn.
-  unfold ITree.map.
-  autorewrite with itree. refl.
-Qed.
 
 
 Definition assumeK E X `{EventE -< E} (P: X -> Prop): ktree E X X :=
