lib/ITreelib.v
@@ -1,0 +1,215 @@
+From ITree Require Export
+     ITree
+     ITreeFacts
+     Events.MapDefault
+     Events.State
+     Events.StateFacts
+     EqAxiom
+.
+From ExtLib Require Export
+     (* Data.String *)
+     (* Structures.Monad *)
+     (* Structures.Traversable *)
+     (* Structures.Foldable *)
+     (* Structures.Reducible *)
+     (* OptionMonad *)
+     Functor FunctorLaws
+     Structures.Maps
+     (* Data.List *)
+.
+From Coq Require Import
+     Arith.PeanoNat
+     (* Strings.String *)
+     Lists.List
+     Morphisms
+     Setoid
+     RelationClasses
+.
+Require Import CoqlibC.
+Require Import Program.
+
+Export SumNotations.
+Export ITreeNotations.
+Export Monads.
+Export MonadNotation.
+Export FunctorNotation.
+Export CatNotations.
+Open Scope cat_scope.
+Open Scope monad_scope.
+Open Scope itree_scope.
+
+
+Set Implicit Arguments.
+
+
+Definition hrespectful A0 A1 B0 B1 (RA: A0 -> A1 -> Prop) (RB: B0 -> B1 -> Prop):
+  (A0 -> B0) -> (A1 -> B1) -> Prop :=
+  fun f0 f1 => forall a0 a1, RA a0 a1 -> RB (f0 a0) (f1 a1)
+.
+
+Definition hrespectful_respectful A B (RA: relation A) (RB: relation B):
+  @hrespectful A A B B RA RB = @respectful A B RA RB.
+Proof. ss. Qed.
+
+Notation " R !-> R' " := (@hrespectful _ _ _ _ (R%signature) (R'%signature))
+                           (right associativity, at level 55).
+                         (* : signature_scope. *)
+
+Class HProper A0 A1 (R : A0 -> A1 -> Prop) (a0: A0) (a1: A1) : Prop := hproper_prf : R a0 a1.
+
+Program Instance HProper_Proper A RA (a: A) (P: HProper RA a a): Proper RA a.
+
+Hint Unfold hrespectful.
+Hint Unfold HProper.
+
+
+
+
+
+Global Instance function_Map (K V: Type) (dec: forall k0 k1, {k0=k1} + {k0<>k1}): (Map K V (K -> option V)) :=
+  Build_Map
+    (fun _ => None)
+    (fun k0 v m => fun k1 => if dec k0 k1 then Some v else m k1)
+    (fun k0 m => fun k1 => if dec k0 k1 then None else m k1)
+    (fun k m => m k)
+    (fun m0 m1 => fun k => match (m0 k) with
+                           | Some v => Some v
+                           | _ => m1 k
+                           end)
+.
+
+(* Lemma eq_eutt *)
+(*       E R *)
+(*       (a b: itree E R) *)
+(*       (EQ: a = b) *)
+(*   : *)
+(*     eutt eq a b *)
+(* . *)
+(* Proof. i. clarify. refl. Qed. *)
+
+(* Lemma vis_not_ret *)
+(*       E R (r: R) X (e: E X) k *)
+(*       (EUTT: Vis e k ≈ Ret r) *)
+(*   : *)
+(*     False *)
+(* . *)
+(* Proof. ii. punfold EUTT. inv EUTT. Qed. *)
+
+
+
+
+
+
+
+
+
+
+
+
+
+Lemma eq_is_bisim: forall E R (t1 t2 : itree E R), t1 = t2 -> t1 ≅ t2.
+Proof. ii. clarify. reflexivity. Qed.
+Lemma bisim_is_eq: forall E R (t1 t2 : itree E R), t1 ≅ t2 -> t1 = t2.
+Proof. ii. eapply bisimulation_is_eq; eauto. Qed.
+
+
+
+Ltac f := first [eapply bisim_is_eq|eapply eq_is_bisim].
+Tactic Notation "f" "in" hyp(H) := first [eapply bisim_is_eq in H|eapply eq_is_bisim in H].
+Ltac ides itr :=
+  let T := fresh "T" in
+  destruct (observe itr) eqn:T;
+  sym in T; apply simpobs in T; apply bisim_is_eq in T; rewrite T in *; clarify.
+Ltac csc := clarify; simpl_depind; clarify.
+
+Notation "tau;; t2" := (Tau t2)
+  (at level 200, right associativity) : itree_scope.
+
+
+
+(*** COPIED FROM MASTER BRANCH. REMOVE LATER ***)
+(*** COPIED FROM MASTER BRANCH. REMOVE LATER ***)
+(*** COPIED FROM MASTER BRANCH. REMOVE LATER ***)
+Lemma eutt_eq_bind : forall E R U (t1 t2: itree E U) (k1 k2: U -> itree E R), t1 ≈ t2 -> (forall u, k1 u ≈ k2 u) -> ITree.bind t1 k1 ≈ ITree.bind t2 k2.
+Proof.
+  intros.
+  eapply eutt_clo_bind with (UU := Logic.eq); [eauto |].
+  intros ? ? ->. apply H0.
+Qed.
+Ltac f_equiv := first [eapply eutt_eq_bind|eapply eqit_VisF|Morphisms.f_equiv].
+(* eapply eqit_bind'| *)
+
+Hint Rewrite @bind_trigger : itree.
+Hint Rewrite @tau_eutt : itree.
+Hint Rewrite @bind_tau : itree.
+
+Tactic Notation "irw" "in" ident(H) := repeat (autorewrite with itree in H; cbn in H).
+Tactic Notation "irw" := repeat (autorewrite with itree; cbn).
+
+(*** TODO: IDK why but (1) ?UNUSNED is needed (2) "fold" tactic does not work. WHY????? ***)
+Ltac fold_eutt :=
+  repeat multimatch goal with
+         | [ H: eqit eq true true ?A ?B |- ?UNUSED ] =>
+           let name := fresh "tmp" in
+           assert(tmp: eutt eq A B) by apply H; clear H; rename tmp into H
+         end
+.
+
+Lemma bind_ret_map {E R1 R2} (u : itree E R1) (f : R1 -> R2) :
+  (r <- u ;; Ret (f r)) ≅ f <$> u.
+Proof.
+  rewrite <- (bind_ret_r u) at 2. apply eqit_bind.
+  - hnf. intros. apply eqit_Ret. auto.
+  - rewrite bind_ret_r. reflexivity.
+Qed.
+
+Lemma map_vis {E R1 R2 X} (e: E X) (k: X -> itree E R1) (f: R1 -> R2) :
+  (* (f <$> (Vis e k)) ≅ Vis e (fun x => f <$> (k x)). *)
+  ITree.map f (Vis e k) ≅ Vis e (fun x => f <$> (k x)).
+Proof.
+  cbn.
+  unfold ITree.map.
+  autorewrite with itree. refl.
+Qed.
+
+
+
+
+(*** TODO: move to SIRCommon ***)
+Lemma unfold_interp_mrec :
+forall (D E : Type -> Type) (ctx : forall T : Type, D T -> itree (D +' E) T) 
+  (R : Type) (t : itree (D +' E) R), interp_mrec ctx t = _interp_mrec ctx (observe t).
+Proof.
+  i. f. eapply unfold_interp_mrec; et.
+Qed.
+
+Lemma bind_ret_l : forall (E : Type -> Type) (R S : Type) (r : R) (k : R -> itree E S),
+    ` x : _ <- Ret r;; k x = k r.
+Proof.
+  i. f. eapply bind_ret_l.
+Qed.
+
+Lemma bind_ret_r : forall (E : Type -> Type) (R : Type) (s : itree E R), ` x : R <- s;; Ret x = s.
+Proof.
+  i. f. eapply bind_ret_r.
+Qed.
+
+Lemma bind_tau : forall (E : Type -> Type) (R U : Type) (t : itree E U) (k : U -> itree E R),
+  ` x : _ <- Tau t;; k x = Tau (` x : _ <- t;; k x).
+Proof.
+  i. f. eapply bind_tau.
+Qed.
+
+Lemma bind_vis: forall (E : Type -> Type) (R U V : Type) (e : E V) (ek : V -> itree E U) (k : U -> itree E R),
+  ` x : _ <- Vis e ek;; k x = Vis e (fun x : V => ` x : _ <- ek x;; k x).
+Proof.
+  i. f. eapply bind_vis.
+Qed.
+
+Lemma bind_trigger: forall (E : Type -> Type) (R U : Type) (e : E U) (k : U -> itree E R),
+    ` x : _ <- ITree.trigger e;; k x = Vis e (fun x : U => k x).
+Proof. i. f. eapply bind_trigger. Qed.
+
+Lemma bind_bind : forall (E : Type -> Type) (R S T : Type) (s : itree E R) (k : R -> itree E S) (h : S -> itree E T),
+    ` x : _ <- (` x : _ <- s;; k x);; h x = ` r : R <- s;; ` x : _ <- k r;; h x.
+Proof. i. f. eapply bind_bind. Qed.
