specIR/SIRmini_stack.v
@@ -15,7 +15,7 @@ Require Import EventsC.
 Require Import GlobalenvsC.
 Require Import IntegersC.
 Require Import Mod ModSem Any Skeleton.
-Require Export SIRCommon2.
+Require Export SIRcommon.
 
 Require Import Program.
 Require Import Simulation.
@@ -53,8 +53,6 @@ Section MODSEM.
   .
 
   Notation update_cur := (fun (st0: state) (cur0: itr) => mk cur0 st0.(cont)).
-
-  Let interp_program0 := interp_program0 p.
 
   Inductive initial_frame (oh0: owned_heap) (args: Args.t): state -> Prop :=
   | initial_frame_intro
